theories/clang/lib/list.v
@@ -28,12 +28,24 @@ Section proof.
       destruct H2 as (?&?&?). by subst.
   Qed.
 
-  Parameter py pt px: addr.
+  Lemma isList_ptr' (l: val) (xs: list val) (t: type) :
+    isList l xs t ⊢ ⌜ typeof l (Tptr (tcell t)) ⌝.
+  Proof.
+    destruct xs as [|x xs'].
+    - iIntros "%". iPureIntro. by subst.
+    - simpl. iIntros "H".
+      iDestruct "H" as (??) "(% & ? & _)".
+      destruct H2 as (?&?&?). by subst.
+  Qed.
+
   Definition x: ident := 1.
   Definition y: ident := 2.
   Definition t: ident := 3.
 
+  Notation "'Tlist'" := (Tptr (tcell Tint32)).
+
   Definition rev_list : expr :=
+    let: t ::: Tptr Tlist := Ealloc (Tptr Tlist) null in
     while [ x != null ] ( x != null ) <{
       t <- snd (!?x) ;;
       snd (!?x) <- y ;;
@@ -41,46 +53,76 @@ Section proof.
       x <- t
     }>.
 
-  Notation "'Tlist'" := (Tptr (tcell Tint32)).
+  Definition ps :=
+    [ (x, Tlist); (y, Tptr Tvoid) ].
 
-  Definition ev : env :=
-    Env [(x, (Tlist, px));
-         (y, (Tptr Tvoid, py));
-         (t, (Tlist, pt))]
-        [].
-
-  Lemma rev_spec Φ body xs:
+  Lemma rev_spec' (f: ident) ks Φ px py pt xs:
     ∀ lx ly ys,
-      instantiate_f_body ev rev_list = Some body →
-      isList lx xs Tint32 ∗ isList ly ys Tint32 ∗ pt ↦ - @ Tlist ∗
-      px ↦ lx @ Tlist ∗ py ↦ ly @ Tptr Tvoid ∗
-      (∀ ly', py ↦ ly' @ Tptr Tvoid ∗ isList ly' (rev xs ++ ys) Tint32 -∗ Φ Vvoid)
-      ⊢ WP body {{ Φ }}.
+      isList lx xs Tint32 ∗
+      isList ly ys Tint32 ∗
+      (∀ ly' : val,
+          isList ly' (rev xs ++ ys) Tint32 -∗ own_stack ([] :: ks) -∗ Φ void) ∗
+      own_stack ([] :: ks) ∗
+      px ↦ lx @ Tlist ∗
+      py ↦ ly @ Tptr Tvoid ∗
+      pt ↦ - @ Tptr Tlist
+  ⊢ WP while [! px @ Tlist != null](! px @ Tlist != null)<{
+     pt <- snd ! ! px @ Tlist @ (tcell Tint32) ;;
+     ! px @ Tlist + Byte.repr 4 <- ! py @ (Tptr Tvoid) ;;
+     py <- ! px @ Tlist ;; px <- ! pt @ (Tptr Tlist) }> {{ v,
+  Φ v }}.
   Proof.
-    unfold_f_inst; destruct px; subst;
-    induction xs as [|x xs' IHxs']; intros ??? [=]; subst.
-    - iIntros "(% & Hlr & Ht & Hpx & Hpy & HΦ)".
-      subst. wp_run.
-      iNext. iApply "HΦ". iFrame.
-    - iIntros "(Hl & Hlr & Ht & Hpx & Hpy & HΦ)".
-      wp_load. iDestruct "Hl" as (p l') "(% & Hp & Hl')".
+    induction xs as [|x xs' IHxs']; intros ??? ; subst.
+    - iIntros "(Hlx & Hly & HΦ & Hs & Hpx & Hpy & Hpt)".
+      iDestruct "Hlx" as "%". wp_run.
+      { by simplify_eq. } wp_run. iNext.
+      iApply ("HΦ" with "[-Hs]")=>//.
+    - iIntros "(Hlx & Hly & HΦ & Hs & Hpx & Hpy & Hpt)".
+      wp_load. iDestruct "Hlx" as (p l') "(% & Hp & Hl')".
       destruct H0 as [? [? ?]]. subst.
       wp_run. iNext. wp_run. iNext.
-      iDestruct "Ht" as (?) "Ht".
+      iDestruct "Hpt" as (?) "Hpt".
       wp_assign. wp_load. destruct p as [pb po]. wp_op.
       rewrite /offset_by_byte.
+      replace (Z.to_nat (Byte.intval (Byte.repr 4))) with 4%nat; last done.
       replace (Z.to_nat (Byte.intval (Byte.repr 4))) with 4%nat; last done. wp_load.
-      iDestruct (isList_ptr with "Hlr") as "%". unfold tcell.
+      iDestruct (isList_ptr with "Hly") as "%". unfold tcell.
       iDestruct (mapstoval_split with "Hp") as "[Hp1 Hp2]". simpl.
       wp_assign. wp_load. wp_assign. wp_load. wp_assign.
-      iApply (IHxs' l' (Vptr (pb, po)) (x::ys)); first by unfold_f_inst.
+      iApply (IHxs' l' (Vptr (pb, po)) (x::ys)).
       iFrame. iDestruct (mapstoval_join with "[Hp1 Hp2]") as "Hp".
       { iSplitL "Hp1"; by simpl. }
-      iSplitL "Hp Hlr".
+      iSplitL "Hp Hly".
       { iExists (pb, po), ly. iFrame.
         iPureIntro. split; [|split]=>//. by eapply typeof_any_ptr. }
-      iSplitL "Ht"; first eauto.
-      by rewrite -app_assoc.
+      iSplitL "HΦ".
+      { by rewrite -app_assoc. } eauto.
+  Qed.
+
+  Lemma rev_spec (f: ident) ks Φ xs:
+    ∀ lx ly ys,
+      text_interp f (Function Tvoid ps rev_list) ∗
+      isList lx xs Tint32 ∗ isList ly ys Tint32 ∗ own_stack ks ∗
+      (∀ ly', isList ly' (rev xs ++ ys) Tint32 -∗ own_stack ([]::ks) -∗ Φ Vvoid)
+      ⊢ WP Ecall_typed Tvoid f [Evalue lx ; Evalue ly] {{ Φ }}.
+  Proof.
+    iIntros (???) "(Hf & Hlx & Hly & Hs & HΦ)". unfold rev_list.
+    iApply (@wp_call _ _ _ [] _ [lx; ly]); last iFrame; first by simpl.
+    iNext. iIntros "Hs'".
+    wp_bind (Ealloc _ _).
+    iDestruct (isList_ptr with "Hly") as "%".
+    iDestruct (isList_ptr' with "Hlx") as "%".
+    iApply wp_alloc=>//. iIntros (px) "Hpx".
+    iApply wp_let=>//.
+    iNext. wp_bind (Ealloc _ _).
+    iApply wp_alloc=>//. iIntros (py) "Hpy".
+    iApply wp_let=>//.
+    iNext.  wp_bind (Ealloc _ _).
+    iApply wp_alloc=>//. iIntros (pt) "Hpt".
+    iApply wp_let=>//.
+    iNext.
+    iApply (rev_spec' f ks Φ px py pt xs lx ly ys). iFrame. eauto.
   Qed.
 
 End proof.
+
