theories/lib/refine_ra.v
@@ -5,7 +5,7 @@ From iris_c.lib Require Import prelude.
 Section algebra.
   Context {spec_state spec_code: Type}.
   Context {spec_step: spec_code → spec_state → spec_code → spec_state → Prop}.
-    
+
   Inductive view : Set := master | snapshot.
 
   Definition max_view (v1 v2: view) :=
